<?xml version="1.0" encoding="utf-8"?>
<rdf:RDF
   xmlns:dcterms="http://purl.org/dc/terms/"
   xmlns:owl="http://www.w3.org/2002/07/owl#"
   xmlns:qb="http://purl.org/linked-data/cube#"
   xmlns:rdf="http://www.w3.org/1999/02/22-rdf-syntax-ns#"
   xmlns:rdfs="http://www.w3.org/2000/01/rdf-schema#"
   xmlns:sdo="https://schema.org/"
   xmlns:sh="http://www.w3.org/ns/shacl#"
   xmlns:skos="http://www.w3.org/2004/02/skos/core#"
   xmlns:vann="http://purl.org/vocab/vann/"
>
  <rdf:Description rdf:about="https://w3id.org/pnv#baseSurname">
    <rdf:type rdf:resource="http://www.w3.org/2002/07/owl#DatatypeProperty"/>
    <rdfs:isDefinedBy rdf:resource="https://w3id.org/pnv#baseSurname"/>
    <skos:definition xml:lang="en">A Base surname is a family name without any prefixes, if those prefixes need to be ignored
                             in sorting. If the family name is e.g. 'de Vries' and it needs to be sorted under 'V',
                             the Base surname is 'Vries'. Base surname is equivalent to BioDes:geslachtsnaam.
                          </skos:definition>
    <rdfs:label xml:lang="en">baseSurname</rdfs:label>
    <sdo:domainIncludes rdf:resource="https://w3id.org/pnv#Name"/>
    <sdo:rangeIncludes rdf:resource="http://www.w3.org/2001/XMLSchema#string"/>
  </rdf:Description>
  <rdf:Description rdf:about="https://personsincontext.org/model/PersonReconstruction">
    <rdf:type rdf:resource="http://www.w3.org/2002/07/owl#Class"/>
    <rdfs:label xml:lang="en">PersonReconstruction</rdfs:label>
    <skos:definition xml:lang="en">A Person reconstruction is the result of modelling one or multiple PersonObservation(s) into a
                           single resource.</skos:definition>
    <skos:scopeNote xml:lang="en">
                            A Person reconstruction must always refer to one or more Person observations. For this,
                            the prov:wasDerivedFrom property is used.
                            Information about the creation should be documented with the prov:wasGeneratedBy property.
                            Information about updates of a Person reconstruction should be documented with
                            prov:wasRevisionOf
                        </skos:scopeNote>
    <rdfs:subClassOf rdf:resource="https://personsincontext.org/model/Person"/>
    <sdo:workExample rdf:nodeID="nf684994b51a046b584742dbc196ee550b5"/>
    <sdo:workExample rdf:nodeID="nf684994b51a046b584742dbc196ee550b6"/>
  </rdf:Description>
  <rdf:Description rdf:nodeID="nf684994b51a046b584742dbc196ee550b7">
    <rdf:type rdf:resource="https://schema.org/ImageObject"/>
    <sh:order rdf:datatype="http://www.w3.org/2001/XMLSchema#integer">0</sh:order>
    <sdo:caption>Schematic overview of a Source</sdo:caption>
    <sdo:contentUrl rdf:datatype="http://www.w3.org/2001/XMLSchema#anyURI">../web_images/pico_source.svg</sdo:contentUrl>
    <sdo:description>Schematic overview of a Source.</sdo:description>
    <sdo:encodingFormat>image/svg+xml</sdo:encodingFormat>
    <sdo:name>Source</sdo:name>
  </rdf:Description>
  <rdf:Description rdf:nodeID="nf684994b51a046b584742dbc196ee550b4">
    <rdf:type rdf:resource="https://schema.org/TextObject"/>
    <sdo:description>Example of two Person Observations from the same source</sdo:description>
    <sdo:encodingFormat>text/turtle</sdo:encodingFormat>
    <sdo:name>Person observation example</sdo:name>
    <sdo:text>
                                            afr:geboorteregiser_1858_po_1
                                               a                     pico:PersonObservation ;
                                               prov:hadPrimarySource afr:geboorteregiser_1858 ;
                                               sdo:name              "Abe Bos" ;
                                               sdo:familyName        "Bos" ;
                                               sdo:givenName         "Abe" ;
                                               sdo:birthDate         "21 Junij 1858"^^xsd:string ;
                                               sdo:birthDate         "1858-06-21"^^xsd:date ;
                                               sdo:birthPlace        "Joure" ;
                                               sdo:gender            sdo:Male ;
                                               pico:hasRole          picot:roles/575 ;  # child
                                               sdo:parent            afr:geboorteregiser_1858_po_2, afr:geboorteregiser_1858_po_3 .

                                            afr:geboorteregiser_1858_po_2
                                               a                     pico:PersonObservation ;
                                               prov:hadPrimarySource afr:geboorteregiser_1858 ;
                                               sdo:name              "Sjouke Abes Bos" ;
                                               sdo:familyName        "Bos" ;
                                               sdo:givenName         "Sjouke" ;
                                               pico:hasAge           "30"^^xsd:decimal ;
                                               sdo:hasOccupation     "klokmakersknecht" ;
                                               sdo:address           "Joure" ;
                                               sdo:gender            sdo:Male ;
                                               sdo:spouse            afr:geboorteregiser_1858_po_3 ;
                                               sdo:children          afr:geboorteregiser_1858_po_1 ;
                                               pico:hasRole          picot:roles/489 .  # declarant
                                         </sdo:text>
  </rdf:Description>
  <rdf:Description rdf:about="https://schema.org/additionalName">
    <rdf:type rdf:resource="http://www.w3.org/2002/07/owl#ObjectProperty"/>
    <rdfs:isDefinedBy rdf:resource="https://schema.org/additionalName"/>
    <skos:definition>The name of a Person, annotated according to the Person Name Vocabulary.</skos:definition>
    <rdfs:label xml:lang="en">additionalName</rdfs:label>
    <sdo:domainIncludes rdf:resource="https://personsincontext.org/model/Person"/>
    <sdo:rangeIncludes rdf:resource="https://w3id.org/pnv#Name"/>
  </rdf:Description>
  <rdf:Description rdf:about="http://www.w3.org/ns/prov#wasDerivedFrom">
    <rdf:type rdf:resource="http://www.w3.org/2002/07/owl#ObjectProperty"/>
    <rdfs:isDefinedBy rdf:resource="http://www.w3.org/ns/prov#wasDerivedFrom"/>
    <skos:definition xml:lang="en">A derivation is a combination of one or more Person observations
                             in a Person reconstruction</skos:definition>
    <rdfs:label xml:lang="en">wasDerivedFrom</rdfs:label>
    <skos:scopeNote xml:lang="en">A PersonReconstruction is always derived from one or more PersonObservations.
                             The wasDerivedFrom property is therefore required for PersonReconstructions.
                          </skos:scopeNote>
    <sdo:domainIncludes rdf:resource="https://personsincontext.org/model/PersonReconstruction"/>
    <sdo:rangeIncludes rdf:resource="https://personsincontext.org/model/PersonObservation"/>
  </rdf:Description>
  <rdf:Description rdf:about="https://schema.org/url">
    <rdf:type rdf:resource="http://www.w3.org/2002/07/owl#ObjectProperty"/>
    <rdfs:isDefinedBy rdf:resource="https://schema.org/url"/>
    <skos:definition>URL of the Source or Scan.</skos:definition>
    <rdfs:label xml:lang="en">url</rdfs:label>
    <skos:scopeNote xml:lang="en">For Sources: a link to the Source at the holding archive. Preferably a permalink.</skos:scopeNote>
    <skos:scopeNote xml:lang="en">For Scans of Sources: a link to the scan of the Source at the holding archive.
                          Preferably a link to a IIIF manifest.
                       </skos:scopeNote>
    <sdo:domainIncludes rdf:resource="https://schema.org/ImageObject"/>
    <sdo:domainIncludes rdf:resource="https://schema.org/ArchiveComponent"/>
    <sdo:rangeIncludes rdf:resource="https://schema.org/URL"/>
  </rdf:Description>
  <rdf:Description rdf:about="https://terms.personsincontext.org/roles">
    <rdf:type rdf:resource="http://www.w3.org/2004/02/skos/core#ConceptScheme"/>
    <rdfs:label>Persons in Context role thesaurus</rdfs:label>
  </rdf:Description>
  <rdf:Description rdf:about="https://w3id.org/pnv#initials">
    <rdf:type rdf:resource="http://www.w3.org/2002/07/owl#DatatypeProperty"/>
    <rdfs:isDefinedBy rdf:resource="https://w3id.org/pnv#initials"/>
    <skos:definition xml:lang="en">An initial is the first letter of a person's given name (or sometimes a combination of
                             letters). The Initials property can be used to separately record the initial(s) of a
                             person's given name(s). Each initial should be followed by a dot. It is recommended to
                             always use the Initials property to record initials, but if only the initials of a given
                             name are known, they may also be recorded using pnv:givenName (or pnv:firstName).
                             Example 1: "Peter R. de Vries" would be modelled using pnv:initials "P.R." and
                             pnv:givenName "Peter R.".
                             Example 2: "C.Joh. Kieviet" would ideally be modelled using pnv:initials "C.Joh.",
                             but pnv:givenName "C.Joh." is also possible.
                             Example 3: "H.A.F.M.O. (Hans) van Mierlo" would be modelled using
                             pnv:initials "H.A.F.M.O." and pnv:givenName "Hans".
                          </skos:definition>
    <rdfs:label xml:lang="en">initials</rdfs:label>
    <sdo:domainIncludes rdf:resource="https://w3id.org/pnv#Name"/>
    <sdo:rangeIncludes rdf:resource="http://www.w3.org/2001/XMLSchema#string"/>
  </rdf:Description>
  <rdf:Description rdf:about="https://personsincontext.org/model/hasDescendant">
    <rdf:type rdf:resource="http://www.w3.org/2002/07/owl#ObjectProperty"/>
    <rdf:type rdf:resource="http://www.w3.org/2002/07/owl#TransitiveProperty"/>
    <rdfs:label xml:lang="en">hasDescendant</rdfs:label>
    <skos:scopeNote xml:lang="en">hasDescendant is not meant to be used as a property for PersonObservations or
                          PersonReconstructions.
                          It is a superclass of hasChild. Since hasAncestor is a owl:TransitiveProperty, this will make
                          the children of your children into your descendants.
                       </skos:scopeNote>
    <rdfs:subPropertyOf rdf:resource="https://schema.org/relatedTo"/>
    <owl:inverseOf rdf:resource="https://personsincontext.org/model/hasAncestor"/>
    <rdfs:domain rdf:resource="https://personsincontext.org/model/Person"/>
    <rdfs:range rdf:resource="https://personsincontext.org/model/Person"/>
  </rdf:Description>
  <rdf:Description rdf:about="https://personsincontext.org/model/hasCousin">
    <rdf:type rdf:resource="http://www.w3.org/2002/07/owl#SymmetricProperty"/>
    <rdf:type rdf:resource="http://www.w3.org/2002/07/owl#ObjectProperty"/>
    <rdfs:label xml:lang="en">hasCousin</rdfs:label>
    <rdfs:subPropertyOf rdf:resource="https://schema.org/relatedTo"/>
    <rdfs:domain rdf:resource="https://personsincontext.org/model/Person"/>
    <rdfs:range rdf:resource="https://personsincontext.org/model/Person"/>
  </rdf:Description>
  <rdf:Description rdf:about="https://w3id.org/pnv#patronym">
    <rdf:type rdf:resource="http://www.w3.org/2002/07/owl#DatatypeProperty"/>
    <rdfs:isDefinedBy rdf:resource="https://w3id.org/pnv#patronym"/>
    <skos:definition>A Patronym is a name element based on the given name of one's father or grandfather.
                             This is also the preferred property for a matronym (i.e. a name element based on the given
                             name of one's mother or grandmother).
                          </skos:definition>
    <rdfs:label xml:lang="en">patronym</rdfs:label>
    <sdo:domainIncludes rdf:resource="https://w3id.org/pnv#Name"/>
    <sdo:rangeIncludes rdf:resource="http://www.w3.org/2001/XMLSchema#string"/>
  </rdf:Description>
  <rdf:Description rdf:nodeID="nf684994b51a046b584742dbc196ee550b8">
    <rdf:type rdf:resource="https://schema.org/TextObject"/>
    <sdo:description>Example of a Source with a linked Scan</sdo:description>
    <sdo:encodingFormat>text/turtle</sdo:encodingFormat>
    <sdo:name>Source with a linked Scan</sdo:name>
    <sdo:text>
                                                   afr:geboorteregiser_1858
                                                       a                   sdo:ArchiveComponent ;
                                                       sdo:additionalType  picot:sourcetypes/551 ;  # civil registry: birth
                                                       sdo:name            "Geboorteregister 1858, archiefnummer 30-16, Burgerlijke Stand Haskerland - Tresoar, inventarisnummer 1020, blad 051" ;
                                                       sdo:holdingArchive  &lt;https://www.tresoar.nl/&gt; ;
                                                       sdo:url             &lt;https://allefriezen.nl/zoeken/deeds/f7e82c08-47c5-de67-c636-26aa1603f6c9&gt; ;
                                                       sdo:dateCreated     "1885"^^xs:gYear ;
                                                       sdo:locationCreated "Haskerland" ;
                                                       sdo:associatedMedia [ a                sdo:ImageObject ;
                                                                             sdo:position  51 ;
                                                                             sdo:url       "https://tresoar-images.memorix.nl/frl/download/fullsize/3a9b2d6a-f225-a14e-ab85-3581be7d4d04.jpg" ;
                                                                             sdo:thumbnail "https://tresoar-images.memorix.nl/frl/thumb/250x250/3a9b2d6a-f225-a14e-ab85-3581be7d4d04.jpg" ; ] .
                                               </sdo:text>
  </rdf:Description>
  <rdf:Description rdf:about="https://schema.org/gender">
    <rdf:type rdf:resource="http://www.w3.org/2002/07/owl#DatatypeProperty"/>
    <rdfs:isDefinedBy rdf:resource="https://schema.org/gender"/>
    <skos:definition>Gender of a Person.</skos:definition>
    <rdfs:label xml:lang="en">gender</rdfs:label>
    <skos:scopeNote xml:lang="en">Use one of: sdo:Male or sdo:Female.</skos:scopeNote>
    <sdo:domainIncludes rdf:resource="https://personsincontext.org/model/Person"/>
    <sdo:rangeIncludes rdf:resource="https://schema.org/GenderType"/>
  </rdf:Description>
  <rdf:Description rdf:about="https://schema.org/additionalType">
    <rdf:type rdf:resource="http://purl.org/linked-data/cube#CodedProperty"/>
    <rdf:type rdf:resource="http://www.w3.org/2002/07/owl#ObjectProperty"/>
    <qb:codeList rdf:resource="https://terms.personsincontext.org/sourcetypes"/>
    <rdfs:isDefinedBy rdf:resource="https://schema.org/additionalType"/>
    <skos:definition>The type of the Source.</skos:definition>
    <rdfs:label xml:lang="en">additionalType</rdfs:label>
    <skos:scopeNote xml:lang="en">Use a term from the PiCo thesaurus for Source types:
                          https://terms.personsincontext.org/sourcetypes
                       </skos:scopeNote>
    <sdo:domainIncludes rdf:resource="https://schema.org/ArchiveComponent"/>
  </rdf:Description>
  <rdf:Description rdf:about="https://personsincontext.org/model/hasUncle_Aunt">
    <rdf:type rdf:resource="http://www.w3.org/2002/07/owl#ObjectProperty"/>
    <rdfs:label xml:lang="en">hasUncle/Aunt</rdfs:label>
    <rdfs:subPropertyOf rdf:resource="https://schema.org/relatedTo"/>
    <rdfs:domain rdf:resource="https://personsincontext.org/model/Person"/>
    <rdfs:range rdf:resource="https://personsincontext.org/model/Person"/>
    <owl:inverseOf rdf:resource="https://personsincontext.org/model/hasNephew_Niece"/>
  </rdf:Description>
  <rdf:Description rdf:about="https://personsincontext.org/model/hasGodchild">
    <rdf:type rdf:resource="http://www.w3.org/2002/07/owl#ObjectProperty"/>
    <rdfs:label xml:lang="en">hasGodchild</rdfs:label>
    <rdfs:subPropertyOf rdf:resource="https://schema.org/relatedTo"/>
    <rdfs:domain rdf:resource="https://personsincontext.org/model/Person"/>
    <rdfs:range rdf:resource="https://personsincontext.org/model/Person"/>
    <owl:inverseOf rdf:resource="https://personsincontext.org/model/hasGodparent"/>
  </rdf:Description>
  <rdf:Description rdf:nodeID="nf684994b51a046b584742dbc196ee550b2">
    <rdf:type rdf:resource="https://schema.org/TextObject"/>
    <sh:order rdf:datatype="http://www.w3.org/2001/XMLSchema#integer">0</sh:order>
    <sdo:encodingFormat>text/turtle</sdo:encodingFormat>
    <sdo:name>Example of an Agent responsible for an Activity</sdo:name>
    <sdo:text>
                                             cbg:reconstruction_activity_01
                                                a                      prov:Activity ;
                                                prov:wasAssociatedWith cbg:reconstruction_agent_01 ;
                                                prov:startedAtTime     "2024-05-24T00:00:00"^^xsd:dateTime ;
                                                prov:endedAtTime       "2024-05-24T00:00:00"^^xsd:dateTime .

                                             cbg:reconstruction_agent_01
                                                a             prov:Agent ;
                                                schema:name   "CBG|Center for Family History" ;
                                                schema:url    &lt;https://cbg.nl&gt; .
                                          </sdo:text>
  </rdf:Description>
  <rdf:Description rdf:about="https://schema.org/ImageObject">
    <rdf:type rdf:resource="http://www.w3.org/2002/07/owl#Class"/>
    <rdfs:subClassOf rdf:resource="https://schema.org/CreativeWork"/>
    <skos:definition xml:lang="en">An image file.</skos:definition>
    <rdfs:label xml:lang="en">Scan</rdfs:label>
    <skos:scopeNote xml:lang="en">A link to the location of the scan at the HoldingArchive.
                        A link to scan as it can be displayed online and a link to a thumbnail (for search results)
                        should be provided. Preferably a link to a IIIF manifest.
                       </skos:scopeNote>
  </rdf:Description>
  <rdf:Description rdf:about="https://personsincontext.org/model/hasRole">
    <rdf:type rdf:resource="http://purl.org/linked-data/cube#CodedProperty"/>
    <rdf:type rdf:resource="http://www.w3.org/2002/07/owl#ObjectProperty"/>
    <qb:codeList rdf:resource="https://terms.personsincontext.org/roles"/>
    <skos:definition>The role of a Person observation on the Source.</skos:definition>
    <rdfs:label xml:lang="en">hasRole</rdfs:label>
    <skos:scopeNote xml:lang="en">Use a term from the PiCo Roles thesaurus:
                          https://terms.personsincontext.org/roles
                       </skos:scopeNote>
    <sdo:domainIncludes rdf:resource="https://personsincontext.org/model/PersonObservation"/>
  </rdf:Description>
  <rdf:Description rdf:about="https://personsincontext.org/model/hasAncestor">
    <rdf:type rdf:resource="http://www.w3.org/2002/07/owl#ObjectProperty"/>
    <rdf:type rdf:resource="http://www.w3.org/2002/07/owl#TransitiveProperty"/>
    <rdfs:label xml:lang="en">hasAncestor</rdfs:label>
    <skos:scopeNote xml:lang="en">hasAncestor is not meant to be used as a property for PersonObservations or
                          PersonReconstructions.
                          It is a superclass of hasParent. Since hasAncestor is a owl:TransitiveProperty, this will make
                          the parent of your parent into your ancestor.
                       </skos:scopeNote>
    <rdfs:subPropertyOf rdf:resource="https://schema.org/relatedTo"/>
    <owl:inverseOf rdf:resource="https://personsincontext.org/model/hasDescendant"/>
    <rdfs:domain rdf:resource="https://personsincontext.org/model/Person"/>
    <rdfs:range rdf:resource="https://personsincontext.org/model/Person"/>
  </rdf:Description>
  <rdf:Description rdf:about="https://personsincontext.org/model/hasFosterChild">
    <rdf:type rdf:resource="http://www.w3.org/2002/07/owl#ObjectProperty"/>
    <rdfs:label xml:lang="en">hasFosterChild</rdfs:label>
    <rdfs:subPropertyOf rdf:resource="https://schema.org/relatedTo"/>
    <rdfs:domain rdf:resource="https://personsincontext.org/model/Person"/>
    <rdfs:range rdf:resource="https://personsincontext.org/model/Person"/>
    <owl:inverseOf rdf:resource="https://personsincontext.org/model/hasFosterParent"/>
  </rdf:Description>
  <rdf:Description rdf:about="https://personsincontext.org/model/hasNephew_Niece">
    <rdf:type rdf:resource="http://www.w3.org/2002/07/owl#ObjectProperty"/>
    <rdfs:label xml:lang="en">hasNephew/Niece</rdfs:label>
    <rdfs:subPropertyOf rdf:resource="https://schema.org/relatedTo"/>
    <rdfs:domain rdf:resource="https://personsincontext.org/model/Person"/>
    <rdfs:range rdf:resource="https://personsincontext.org/model/Person"/>
    <owl:inverseOf rdf:resource="https://personsincontext.org/model/hasUncle_Aunt"/>
  </rdf:Description>
  <rdf:Description rdf:about="https://personsincontext.org/model/hasGodparent">
    <rdf:type rdf:resource="http://www.w3.org/2002/07/owl#ObjectProperty"/>
    <rdfs:label xml:lang="en">hasGodparent</rdfs:label>
    <rdfs:subPropertyOf rdf:resource="https://schema.org/relatedTo"/>
    <rdfs:domain rdf:resource="https://personsincontext.org/model/Person"/>
    <rdfs:range rdf:resource="https://personsincontext.org/model/Person"/>
    <owl:inverseOf rdf:resource="https://personsincontext.org/model/hasGodchild"/>
  </rdf:Description>
  <rdf:Description rdf:about="https://schema.org/name">
    <rdf:type rdf:resource="http://www.w3.org/2002/07/owl#DatatypeProperty"/>
    <rdfs:isDefinedBy rdf:resource="https://schema.org/name"/>
    <skos:definition>The name of a Person or a Source.</skos:definition>
    <rdfs:label xml:lang="en">name</rdfs:label>
    <skos:scopeNote xml:lang="en">For Persons: Use full name if the name can't be split into given name and family name.
                          Otherwise use sdo:givenNamen and sdo:fullName or the more extensive pnv:Name.
                       </skos:scopeNote>
    <skos:scopeNote xml:lang="en">For Sources: Use a user-friendly name to identify the source. Depending on the Source type,
                          this may contain a combination of it's name, year of creation, creator, et cetera.
                       </skos:scopeNote>
    <sdo:domainIncludes rdf:resource="https://personsincontext.org/model/Person"/>
    <sdo:domainIncludes rdf:resource="https://schema.org/ArchiveComponent"/>
    <sdo:rangeIncludes rdf:resource="http://www.w3.org/2001/XMLSchema#string"/>
  </rdf:Description>
  <rdf:Description rdf:about="http://www.w3.org/ns/prov#startedAtTime">
    <rdf:type rdf:resource="http://www.w3.org/2002/07/owl#DatatypeProperty"/>
    <rdfs:isDefinedBy rdf:resource="http://www.w3.org/ns/prov#startedAtTime"/>
    <skos:definition>The start time of the activity that generated a Person Reconstruction.</skos:definition>
    <rdfs:label>startedAtTime</rdfs:label>
    <sdo:domainIncludes rdf:resource="http://www.w3.org/ns/prov#Activity"/>
    <sdo:rangeIncludes rdf:resource="http://www.w3.org/2001/XMLSchema#dateTime"/>
  </rdf:Description>
  <rdf:Description rdf:about="https://schema.org/spouse">
    <rdf:type rdf:resource="http://www.w3.org/2002/07/owl#ObjectProperty"/>
    <rdf:type rdf:resource="http://www.w3.org/2002/07/owl#SymmetricProperty"/>
    <rdfs:isDefinedBy rdf:resource="https://schema.org/spouse"/>
    <skos:definition xml:lang="en">The person's spouse.</skos:definition>
    <rdfs:label xml:lang="en">spouse</rdfs:label>
    <skos:scopeNote xml:lang="en">For Person observations, the spouse should always refer to another Person observation
                             on the same Source.
                          </skos:scopeNote>
    <skos:scopeNote xml:lang="en">For Person reconstructions, the spouse should refer to the Person reconstruction of
                             the spouse.
                          </skos:scopeNote>
    <rdfs:subPropertyOf rdf:resource="https://schema.org/relatedTo"/>
    <sdo:domainIncludes rdf:resource="https://personsincontext.org/model/Person"/>
    <sdo:rangeIncludes rdf:resource="https://personsincontext.org/model/Person"/>
  </rdf:Description>
  <rdf:Description rdf:about="https://personsincontext.org/model/hasStepchild-in-law">
    <rdf:type rdf:resource="http://www.w3.org/2002/07/owl#ObjectProperty"/>
    <rdfs:label xml:lang="en">hasStepchild-in-law</rdfs:label>
    <rdfs:subPropertyOf rdf:resource="https://schema.org/relatedTo"/>
    <rdfs:domain rdf:resource="https://personsincontext.org/model/Person"/>
    <rdfs:range rdf:resource="https://personsincontext.org/model/Person"/>
    <owl:inverseOf rdf:resource="https://personsincontext.org/model/hasStepparent-in-law"/>
  </rdf:Description>
  <rdf:Description rdf:about="https://schema.org/embedUrl">
    <rdf:type rdf:resource="http://www.w3.org/2002/07/owl#ObjectProperty"/>
    <rdfs:isDefinedBy rdf:resource="https://schema.org/embedUrl"/>
    <skos:definition xml:lang="en">A URL pointing to a viewer for a specific scan.</skos:definition>
    <rdfs:label xml:lang="en">embedUrl</rdfs:label>
    <sdo:domainIncludes rdf:resource="https://schema.org/ImageObject"/>
    <sdo:rangeIncludes rdf:resource="https://schema.org/URL"/>
  </rdf:Description>
  <rdf:Description rdf:about="https://schema.org/address">
    <rdf:type rdf:resource="http://www.w3.org/2002/07/owl#DatatypeProperty"/>
    <rdfs:isDefinedBy rdf:resource="https://schema.org/address"/>
    <skos:definition>Physical address of the Person.</skos:definition>
    <rdfs:label xml:lang="en">address</rdfs:label>
    <skos:scopeNote xml:lang="en">Address of a Person as mentioned on the Source.</skos:scopeNote>
    <sdo:domainIncludes rdf:resource="https://personsincontext.org/model/PersonObservation"/>
    <sdo:rangeIncludes rdf:resource="https://schema.org/Text"/>
  </rdf:Description>
  <rdf:Description rdf:about="https://personsincontext.org/model/hasGreat-grandparent">
    <rdf:type rdf:resource="http://www.w3.org/2002/07/owl#ObjectProperty"/>
    <rdfs:label xml:lang="en">hasGreat-grandparent</rdfs:label>
    <rdfs:subPropertyOf rdf:resource="https://schema.org/relatedTo"/>
    <rdfs:domain rdf:resource="https://personsincontext.org/model/Person"/>
    <rdfs:range rdf:resource="https://personsincontext.org/model/Person"/>
    <owl:inverseOf rdf:resource="https://personsincontext.org/model/hasGreat-grandchild"/>
  </rdf:Description>
  <rdf:Description rdf:about="http://www.w3.org/ns/prov#wasGeneratedBy">
    <rdf:type rdf:resource="http://www.w3.org/2002/07/owl#ObjectProperty"/>
    <rdfs:isDefinedBy rdf:resource="http://www.w3.org/ns/prov#wasGeneratedBy"/>
    <skos:definition xml:lang="en">Generation is the completion of production of a new Person reconstruction by an activity.
                          This Person reconstruction did not exist before generation and becomes available
                          for usage after this generation.
                       </skos:definition>
    <rdfs:label xml:lang="en">wasGeneratedBy</rdfs:label>
    <skos:scopeNote xml:lang="en">Required for PersonReconstructions.</skos:scopeNote>
    <sdo:domainIncludes rdf:resource="https://personsincontext.org/model/PersonReconstruction"/>
    <sdo:rangeIncludes rdf:resource="http://www.w3.org/ns/prov#Activity"/>
  </rdf:Description>
  <rdf:Description rdf:about="http://www.w3.org/ns/prov#endedAtTime">
    <rdf:type rdf:resource="http://www.w3.org/2002/07/owl#DatatypeProperty"/>
    <rdfs:isDefinedBy rdf:resource="http://www.w3.org/ns/prov#endedAtTime"/>
    <skos:definition>The end time of the activity that generated a Person Reconstruction.</skos:definition>
    <rdfs:label>endedAtTime</rdfs:label>
    <sdo:domainIncludes rdf:resource="http://www.w3.org/ns/prov#Activity"/>
    <sdo:rangeIncludes rdf:resource="http://www.w3.org/2001/XMLSchema#dateTime"/>
  </rdf:Description>
  <rdf:Description rdf:about="https://schema.org/ArchiveComponent">
    <rdf:type rdf:resource="http://www.w3.org/2002/07/owl#Class"/>
    <rdfs:subClassOf rdf:resource="https://schema.org/CreativeWork"/>
    <skos:definition xml:lang="en">An intangible type to be applied to any archive content, carrying with it a set of
                            properties required to describe archival items and collections.</skos:definition>
    <rdfs:label xml:lang="en">Source</rdfs:label>
    <skos:scopeNote xml:lang="en">Person observations can appear on many types of historical documents. The PiCo model does
                          not aim to describe these sources, as excellent data models, such as Records in Contexts and
                          Dublin Core, already exist within the heritage domain. In order to model person observations,
                          we require that institutions describe their sources at least with a single name property that
                          combines identifying information about the source like its title and creation date.
                          For example, a Marriage Certificate is then described as follows: "BS Marriage Haarlem,
                          November 11, 1885, certificate number 321". As long as this description consists of various
                          elements that identify the source, heritage institutions are free to use any authoritative
                          domain-specific standard to describe their historical person records.
                       </skos:scopeNote>
    <sdo:workExample rdf:nodeID="nf684994b51a046b584742dbc196ee550b7"/>
    <sdo:workExample rdf:nodeID="nf684994b51a046b584742dbc196ee550b8"/>
  </rdf:Description>
  <rdf:Description rdf:about="https://personsincontext.org/model/hasGrandparent-in-law">
    <rdf:type rdf:resource="http://www.w3.org/2002/07/owl#ObjectProperty"/>
    <rdfs:label xml:lang="en">hasGrandparent-in-law</rdfs:label>
    <rdfs:subPropertyOf rdf:resource="https://schema.org/relatedTo"/>
    <rdfs:domain rdf:resource="https://personsincontext.org/model/Person"/>
    <rdfs:range rdf:resource="https://personsincontext.org/model/Person"/>
    <owl:inverseOf rdf:resource="https://personsincontext.org/model/hasGrandchild-in-law"/>
  </rdf:Description>
  <rdf:Description rdf:about="https://personsincontext.org/model/PersonObservation">
    <rdf:type rdf:resource="http://www.w3.org/2002/07/owl#Class"/>
    <rdfs:label xml:lang="en">PersonObservation</rdfs:label>
    <skos:definition xml:lang="en">A Person observation is a person that can be observed on a Source</skos:definition>
    <skos:scopeNote xml:lang="en">A person observation represents how a person is recorded on a Source. Therefore, it must
                       always be related to a source. Person observations closely reflect data as it appears in the
                       source, that is, with the age, occupation, and spelling of the person's name recorded as in the
                       record. A notable exception are dates where the creator of the person observation is encouraged
                       to write down the date according to the YMD ISO 8601 date standard (for example: '1802-07-29'),
                       even though the source probably lists the date in a DMY or MDY format or another calendar
                       entirely. Information on the original entry can be stored using an optional triple.
                    </skos:scopeNote>
    <rdfs:subClassOf rdf:resource="https://personsincontext.org/model/Person"/>
    <sdo:workExample rdf:nodeID="nf684994b51a046b584742dbc196ee550b3"/>
    <sdo:workExample rdf:nodeID="nf684994b51a046b584742dbc196ee550b4"/>
  </rdf:Description>
  <rdf:Description rdf:about="https://personsincontext.org/model/hasPreviousPartner">
    <rdf:type rdf:resource="http://www.w3.org/2002/07/owl#SymmetricProperty"/>
    <rdf:type rdf:resource="http://www.w3.org/2002/07/owl#ObjectProperty"/>
    <rdfs:label xml:lang="en">hasPreviousPartner</rdfs:label>
    <rdfs:subPropertyOf rdf:resource="https://schema.org/relatedTo"/>
    <rdfs:domain rdf:resource="https://personsincontext.org/model/Person"/>
    <rdfs:range rdf:resource="https://personsincontext.org/model/Person"/>
  </rdf:Description>
  <rdf:Description rdf:nodeID="nf684994b51a046b584742dbc196ee550b5">
    <rdf:type rdf:resource="https://schema.org/ImageObject"/>
    <sh:order rdf:datatype="http://www.w3.org/2001/XMLSchema#integer">0</sh:order>
    <sdo:caption>Schematic overview of a person reconstruction</sdo:caption>
    <sdo:contentUrl rdf:datatype="http://www.w3.org/2001/XMLSchema#anyURI">../web_images/pico_personreconstruction.svg</sdo:contentUrl>
    <sdo:description>Schematic overview of a person reconstruction.</sdo:description>
    <sdo:encodingFormat>image/svg+xml</sdo:encodingFormat>
    <sdo:name>PersonReconstruction overview</sdo:name>
  </rdf:Description>
  <rdf:Description rdf:about="http://www.w3.org/ns/prov#wasAssociatedWith">
    <rdf:type rdf:resource="http://www.w3.org/2002/07/owl#DatatypeProperty"/>
    <rdfs:isDefinedBy rdf:resource="http://www.w3.org/ns/prov#wasAssociatedWith"/>
    <skos:definition xml:lang="en">Assignment of responsibility to an agent for the activity of creating a person reconstruction.</skos:definition>
    <rdfs:label>wasAssociatedWith</rdfs:label>
    <sdo:domainIncludes rdf:resource="http://www.w3.org/ns/prov#Activity"/>
    <sdo:rangeIncludes rdf:resource="http://www.w3.org/ns/prov#Agent"/>
  </rdf:Description>
  <rdf:Description rdf:nodeID="nf684994b51a046b584742dbc196ee550b3">
    <rdf:type rdf:resource="https://schema.org/ImageObject"/>
    <sh:order rdf:datatype="http://www.w3.org/2001/XMLSchema#integer">0</sh:order>
    <sdo:caption>Schematic overview of a PersonObservation</sdo:caption>
    <sdo:contentUrl rdf:datatype="http://www.w3.org/2001/XMLSchema#anyURI">../web_images/pico_personobservation.svg</sdo:contentUrl>
    <sdo:description>Schematic overview of a person observation.</sdo:description>
    <sdo:encodingFormat>image/svg+xml</sdo:encodingFormat>
    <sdo:name>PersonObservation overview</sdo:name>
  </rdf:Description>
  <rdf:Description rdf:about="https://schema.org/thumbnail">
    <rdf:type rdf:resource="http://www.w3.org/2002/07/owl#ObjectProperty"/>
    <skos:definition xml:lang="en">Thumbnail image of the Scan.</skos:definition>
    <rdfs:label xml:lang="en">thumbnail</rdfs:label>
    <sdo:domainIncludes rdf:resource="https://schema.org/ImageObject"/>
    <sdo:rangeIncludes rdf:resource="https://schema.org/ImageObject"/>
  </rdf:Description>
  <rdf:Description rdf:about="https://personsincontext.org/model/hasReligion">
    <rdf:type rdf:resource="http://www.w3.org/2002/07/owl#DatatypeProperty"/>
    <skos:definition>Religious conviction related to a person in an observation.</skos:definition>
    <rdfs:label>hasReligion</rdfs:label>
    <skos:scopeNote xml:lang="en">Religion as mentioned on the Source.
                         If desired, a SKOS thesaurus can be used to annotate religion.
                      </skos:scopeNote>
    <rdfs:domain rdf:resource="https://personsincontext.org/model/Person"/>
    <sdo:rangeIncludes rdf:resource="http://www.w3.org/2001/XMLSchema#string"/>
    <sdo:rangeIncludes rdf:resource="http://www.w3.org/2001/XMLSchema#anyURI"/>
  </rdf:Description>
  <rdf:Description rdf:about="http://www.w3.org/ns/prov#Activity">
    <rdf:type rdf:resource="http://www.w3.org/2002/07/owl#Class"/>
    <rdfs:label xml:lang="en">Activity</rdfs:label>
    <skos:definition>The Activity that generated a PersonReconstruction</skos:definition>
    <skos:scopeNote xml:lang="en">A Person Reconstruction can either be created by a human researcher or by a software algorithm.
                       In case of a human-made reconstruction, provide information about the time, place and knowledge-
                       input. In case of a software algorithm, provide information about the name, version and
                       configuration settings of the program.
                    </skos:scopeNote>
  </rdf:Description>
  <rdf:Description rdf:about="https://personsincontext.org/model/hasLegitimizedChild">
    <rdf:type rdf:resource="http://www.w3.org/2002/07/owl#ObjectProperty"/>
    <rdfs:label xml:lang="en">hasLegitimizedChild</rdfs:label>
    <rdfs:subPropertyOf rdf:resource="https://schema.org/relatedTo"/>
    <rdfs:domain rdf:resource="https://personsincontext.org/model/Person"/>
    <rdfs:range rdf:resource="https://personsincontext.org/model/Person"/>
    <owl:inverseOf rdf:resource="https://personsincontext.org/model/isLegitimitezedChildOf"/>
  </rdf:Description>
  <rdf:Description rdf:about="https://schema.org/deathPlace">
    <rdf:type rdf:resource="http://www.w3.org/2002/07/owl#DatatypeProperty"/>
    <rdfs:isDefinedBy rdf:resource="https://schema.org/deathPlace"/>
    <skos:definition xml:lang="en">The place where the person died.</skos:definition>
    <skos:scopeNote xml:lang="en">Preferably, use a link to an existing thesaurus like geonames or wikidata.
                          If desired, both the literal place, as mentioned on the Source can be used together with
                          the reconciled version.
                       </skos:scopeNote>
    <rdfs:label xml:lang="en">deathPlace</rdfs:label>
    <sdo:domainIncludes rdf:resource="https://personsincontext.org/model/Person"/>
    <sdo:rangeIncludes rdf:resource="http://www.w3.org/2001/XMLSchema#string"/>
    <sdo:rangeIncludes rdf:resource="http://www.w3.org/2001/XMLSchema#anyURI"/>
  </rdf:Description>
  <rdf:Description rdf:about="https://personsincontext.org/model/hasUncle_Aunt-in-law">
    <rdf:type rdf:resource="http://www.w3.org/2002/07/owl#ObjectProperty"/>
    <rdfs:label>hasUncle/Aunt-in-law</rdfs:label>
    <rdfs:subPropertyOf rdf:resource="https://schema.org/relatedTo"/>
    <rdfs:domain rdf:resource="https://personsincontext.org/model/Person"/>
    <rdfs:range rdf:resource="https://personsincontext.org/model/Person"/>
    <owl:inverseOf rdf:resource="https://personsincontext.org/model/hasNephew_Niece-in-law"/>
  </rdf:Description>
  <rdf:Description rdf:about="https://schema.org/deathDate">
    <rdf:type rdf:resource="http://www.w3.org/2002/07/owl#DatatypeProperty"/>
    <rdfs:isDefinedBy rdf:resource="https://schema.org/deathDate"/>
    <skos:definition>Date of death.</skos:definition>
    <rdfs:label xml:lang="en">deathDate</rdfs:label>
    <skos:scopeNote xml:lang="en">The death date of a person. A date value in ISO 8601 format should be used.
                             Incomplete dates are allowed, but only when truncated from small to large. For example:
                             "1970-08-15", "1970-08" and "1970" are all allowed, but "1970-00-15" or "08-15" are not.
                             When the date of death is not known, but is known that a person is deceased, the
                             property pico:deceased can be used.
                             Sometimes, you may want to use a string as deathDate. For example if you want to or have to
                             record the date exactly as it was written on the Source. If possible use both the string
                             format and the xsd:date format in this case.
                          </skos:scopeNote>
    <sdo:domainIncludes rdf:resource="https://personsincontext.org/model/Person"/>
    <sdo:rangeIncludes rdf:resource="http://www.w3.org/2001/XMLSchema#date"/>
    <sdo:rangeIncludes rdf:resource="http://www.w3.org/2001/XMLSchema#string"/>
  </rdf:Description>
  <rdf:Description rdf:about="https://schema.org/position">
    <rdf:type rdf:resource="http://www.w3.org/2002/07/owl#DatatypeProperty"/>
    <rdfs:isDefinedBy rdf:resource="https://schema.org/position"/>
    <skos:definition>The position of the scan in the order of a set of scans</skos:definition>
    <rdfs:label xml:lang="en">position</rdfs:label>
    <skos:scopeNote xml:lang="en">The position defines the order in which scans are presented on the web.
                          This feature is required when a Source has multiple scans.
                       </skos:scopeNote>
    <sdo:domainIncludes rdf:resource="https://schema.org/ImageObject"/>
    <sdo:rangeIncludes rdf:resource="http://www.w3.org/2001/XMLSchema#int"/>
  </rdf:Description>
  <rdf:Description rdf:about="https://schema.org/contentLocation">
    <rdf:type rdf:resource="http://www.w3.org/2002/07/owl#DatatypeProperty"/>
    <rdfs:isDefinedBy rdf:resource="https://schema.org/contentLocation"/>
    <skos:definition xml:lang="en">The location depicted or described in the content.
                          For example, the geographic coverage of an archival record.
                          Or the location in a photograph or painting.
                       </skos:definition>
    <rdfs:label xml:lang="en">contentLocation</rdfs:label>
    <sdo:domainIncludes rdf:resource="https://schema.org/ArchiveComponent"/>
    <sdo:rangeIncludes rdf:resource="http://www.w3.org/2001/XMLSchema#string"/>
    <sdo:rangeIncludes rdf:resource="http://www.w3.org/2001/XMLSchema#anyURI"/>
  </rdf:Description>
  <rdf:Description rdf:about="https://personsincontext.org/model/Person">
    <rdf:type rdf:resource="http://www.w3.org/2002/07/owl#Class"/>
    <rdfs:label xml:lang="en">Person</rdfs:label>
    <skos:definition xml:lang="en">A Person is a human being whose individual existence can somehow be documented.</skos:definition>
    <skos:scopeNote xml:lang="en">Container class for Person observation and Person reconstruction. Not to be used directly in
                       PiCo resources.
                    </skos:scopeNote>
    <rdfs:subClassOf rdf:resource="https://w3id.org/pnv#Person"/>
    <rdfs:subClassOf rdf:resource="http://www.w3.org/ns/prov#Entity"/>
  </rdf:Description>
  <rdf:Description rdf:about="http://www.w3.org/ns/prov#hadPrimarySource">
    <rdf:type rdf:resource="http://www.w3.org/2002/07/owl#ObjectProperty"/>
    <rdfs:isDefinedBy rdf:resource="http://www.w3.org/ns/prov#hadPrimarySource"/>
    <skos:definition xml:lang="en">A primary source for a topic refers to something produced by some agent with direct
                             experience and knowledge about the topic, at the time of the topic's study, without
                             benefit from hindsight. Because of the directness of primary sources, they
                             'speak for themselves' in ways that cannot be captured through the filter of secondary
                             sources. As such, it is important for secondary sources to reference those primary
                             sources from which they were derived, so that their reliability can be investigated.
                             A primary source relation is a particular case of derivation of secondary materials from
                             their primary sources. It is recognized that the determination of primary sources can be
                             up to interpretation, and should be done according to conventions accepted within the
                             application's domain.
                          </skos:definition>
    <rdfs:label xml:lang="en">hadPrimarySource</rdfs:label>
    <skos:scopeNote>Linking a Source with the hadPrimarySource property is required for Person Observations.</skos:scopeNote>
    <sdo:domainIncludes rdf:resource="https://personsincontext.org/model/PersonObservation"/>
    <sdo:rangeIncludes rdf:resource="https://schema.org/ArchiveComponent"/>
  </rdf:Description>
  <rdf:Description rdf:about="https://schema.org/holdingArchive">
    <rdf:type rdf:resource="http://www.w3.org/2002/07/owl#ObjectProperty"/>
    <rdfs:isDefinedBy rdf:resource="https://schema.org/holdingArchive"/>
    <skos:definition>Organization that holds, keeps or maintains the ArchiveComponent.</skos:definition>
    <rdfs:label xml:lang="en">holdingArchive</rdfs:label>
    <skos:scopeNote>Todo</skos:scopeNote>
    <sdo:domainIncludes rdf:resource="https://schema.org/ArchiveComponent"/>
    <sdo:rangeIncludes rdf:resource="http://www.w3.org/2001/XMLSchema#anyURI"/>
  </rdf:Description>
  <rdf:Description rdf:about="https://personsincontext.org/model/hasFosterParent">
    <rdf:type rdf:resource="http://www.w3.org/2002/07/owl#ObjectProperty"/>
    <rdfs:label xml:lang="en">hasFosterParent</rdfs:label>
    <rdfs:subPropertyOf rdf:resource="https://schema.org/relatedTo"/>
    <rdfs:domain rdf:resource="https://personsincontext.org/model/Person"/>
    <rdfs:range rdf:resource="https://personsincontext.org/model/Person"/>
    <owl:inverseOf rdf:resource="https://personsincontext.org/model/hasFosterChild"/>
  </rdf:Description>
  <rdf:Description rdf:about="https://schema.org/sibling">
    <rdf:type rdf:resource="http://www.w3.org/2002/07/owl#ObjectProperty"/>
    <rdf:type rdf:resource="http://www.w3.org/2002/07/owl#SymmetricProperty"/>
    <rdfs:isDefinedBy rdf:resource="https://schema.org/sibling"/>
    <skos:definition xml:lang="en">A person's brother or sister.</skos:definition>
    <rdfs:label xml:lang="en">sibling</rdfs:label>
    <skos:scopeNote xml:lang="en">For Person observations, the sibling should always refer to another Person observation
                             on the same Source.
                          </skos:scopeNote>
    <skos:scopeNote xml:lang="en">For Person reconstructions, the sibling should refer to the Person reconstruction of
                             the spouse.
                          </skos:scopeNote>
    <rdfs:subPropertyOf rdf:resource="https://schema.org/relatedTo"/>
    <sdo:domainIncludes rdf:resource="https://personsincontext.org/model/Person"/>
    <sdo:rangeIncludes rdf:resource="https://personsincontext.org/model/Person"/>
  </rdf:Description>
  <rdf:Description rdf:about="https://personsincontext.org/model/hasGrandchild">
    <rdf:type rdf:resource="http://www.w3.org/2002/07/owl#ObjectProperty"/>
    <rdfs:label xml:lang="en">hasGrandchild</rdfs:label>
    <rdfs:subPropertyOf rdf:resource="https://schema.org/relatedTo"/>
    <rdfs:domain rdf:resource="https://personsincontext.org/model/Person"/>
    <rdfs:range rdf:resource="https://personsincontext.org/model/Person"/>
    <owl:inverseOf rdf:resource="https://personsincontext.org/model/hasGrandparent"/>
  </rdf:Description>
  <rdf:Description rdf:about="https://personsincontext.org/model/isLegitimitezedChildOf">
    <rdf:type rdf:resource="http://www.w3.org/2002/07/owl#ObjectProperty"/>
    <rdfs:label>isLegitimitezedChildOf</rdfs:label>
    <rdfs:subPropertyOf rdf:resource="https://schema.org/relatedTo"/>
    <rdfs:domain rdf:resource="https://personsincontext.org/model/Person"/>
    <rdfs:range rdf:resource="https://personsincontext.org/model/Person"/>
    <owl:inverseOf rdf:resource="https://personsincontext.org/model/hasLegitimizedChild"/>
  </rdf:Description>
  <rdf:Description rdf:about="http://www.w3.org/ns/prov#Agent">
    <rdf:type rdf:resource="http://www.w3.org/2002/07/owl#Class"/>
    <rdfs:label xml:lang="en">Agent</rdfs:label>
    <skos:definition>The agent (person or organisation) that is responsible for the creation of a person reconstruction.</skos:definition>
    <sdo:workExample rdf:nodeID="nf684994b51a046b584742dbc196ee550b2"/>
  </rdf:Description>
  <rdf:Description rdf:about="https://personsincontext.org/model/isWidOf">
    <rdf:type rdf:resource="http://www.w3.org/2002/07/owl#ObjectProperty"/>
    <rdfs:label xml:lang="en">isWidow/WidowerOf</rdfs:label>
    <rdfs:subPropertyOf rdf:resource="https://schema.org/relatedTo"/>
    <rdfs:domain rdf:resource="https://personsincontext.org/model/Person"/>
    <rdfs:range rdf:resource="https://personsincontext.org/model/Person"/>
  </rdf:Description>
  <rdf:Description rdf:about="https://personsincontext.org/model/hasCousin-in-law">
    <rdf:type rdf:resource="http://www.w3.org/2002/07/owl#SymmetricProperty"/>
    <rdf:type rdf:resource="http://www.w3.org/2002/07/owl#ObjectProperty"/>
    <rdfs:label xml:lang="en">hasCousin-in-law</rdfs:label>
    <rdfs:subPropertyOf rdf:resource="https://schema.org/relatedTo"/>
    <rdfs:domain rdf:resource="https://personsincontext.org/model/Person"/>
    <rdfs:range rdf:resource="https://personsincontext.org/model/Person"/>
  </rdf:Description>
  <rdf:Description rdf:about="https://personsincontext.org/model">
    <rdf:type rdf:resource="http://www.w3.org/2002/07/owl#Ontology"/>
    <rdfs:label xml:lang="en">Persons in Context</rdfs:label>
    <sdo:publisher rdf:resource="https://cbg.nl"/>
    <dcterms:creator>Jeroen Balkenende</dcterms:creator>
    <dcterms:creator>Bob Coret</dcterms:creator>
    <dcterms:creator>Mark Lindeman</dcterms:creator>
    <dcterms:creator>Pieter Woltjer</dcterms:creator>
    <dcterms:creator>Ivo Zandhuis</dcterms:creator>
    <dcterms:contributor>Rick Companje</dcterms:contributor>
    <dcterms:contributor>Rick Mourits</dcterms:contributor>
    <dcterms:contributor>Micon Schorsij</dcterms:contributor>
    <dcterms:contributor>Richard Zijdeman</dcterms:contributor>
    <dcterms:created rdf:datatype="http://www.w3.org/2001/XMLSchema#date">2023-09-21</dcterms:created>
    <dcterms:modified rdf:datatype="http://www.w3.org/2001/XMLSchema#date">2024-04-25</dcterms:modified>
    <dcterms:license rdf:datatype="http://www.w3.org/2001/XMLSchema#anyURI">https://creativecommons.org/licenses/by-sa/4.0/</dcterms:license>
    <dcterms:rights rdf:resource="https://cbg.nl"/>
    <owl:versionInfo xml:lang="en">0.9 - First published version of the PiCo model.</owl:versionInfo>
    <vann:preferredNamespacePrefix>pico</vann:preferredNamespacePrefix>
    <skos:definition xml:lang="en">Persons in Context, abbreviated as PiCo, is a knowledge model for annotating and
                                     publishing person observations from historical sources.
                                     A main characteristic of PiCo is the distinction between Person observations
                                     (person data as found on a Source) and Person reconstructions
                                     (groupings of Person observations, created by the process of matching Person
                                     observations).
                                     PiCo makes use of existing ontologies where possible and adds its own classes
                                     and properties when required.
                                  </skos:definition>
    <skos:historyNote xml:lang="en">
                                     Persons in Context is developed by the CBG|Center for family
                                     history as a successor of the XML standard A2A for annotating historical person
                                     data. Cultural heritage institutions in the Netherlands are encouraged to move to
                                     PiCo.
                                     PiCo was developed in collaboration with technical and domain experts.
                                     The first version of PiCo was reviewed by a selected group of Dutch archivists and
                                     scientists. PiCo is maintained by the PiCo Maintenance Group.
                                  </skos:historyNote>
    <sdo:codeRepository rdf:datatype="http://www.w3.org/2001/XMLSchema#anyURI">https://github.com/CBG-Centrum-voor-familiegeschiedenis/PiCo/</sdo:codeRepository>
    <sdo:workExample rdf:nodeID="nf684994b51a046b584742dbc196ee550b1"/>
  </rdf:Description>
  <rdf:Description rdf:about="https://personsincontext.org/model/hasSibling-in-law">
    <rdf:type rdf:resource="http://www.w3.org/2002/07/owl#SymmetricProperty"/>
    <rdf:type rdf:resource="http://www.w3.org/2002/07/owl#ObjectProperty"/>
    <rdfs:label xml:lang="en">hasSibling-in-law</rdfs:label>
    <rdfs:subPropertyOf rdf:resource="https://schema.org/relatedTo"/>
    <rdfs:domain rdf:resource="https://personsincontext.org/model/Person"/>
    <rdfs:range rdf:resource="https://personsincontext.org/model/Person"/>
  </rdf:Description>
  <rdf:Description rdf:about="https://personsincontext.org/model/hasHalf-sibling">
    <rdf:type rdf:resource="http://www.w3.org/2002/07/owl#SymmetricProperty"/>
    <rdf:type rdf:resource="http://www.w3.org/2002/07/owl#ObjectProperty"/>
    <rdfs:label xml:lang="en">hasHalf-sibling</rdfs:label>
    <rdfs:subPropertyOf rdf:resource="https://schema.org/relatedTo"/>
    <rdfs:domain rdf:resource="https://personsincontext.org/model/Person"/>
    <rdfs:range rdf:resource="https://personsincontext.org/model/Person"/>
  </rdf:Description>
  <rdf:Description rdf:about="https://schema.org/birthPlace">
    <rdf:type rdf:resource="http://www.w3.org/2002/07/owl#DatatypeProperty"/>
    <rdfs:isDefinedBy rdf:resource="https://schema.org/birthPlace"/>
    <skos:definition>The place where a person was born.</skos:definition>
    <rdfs:label xml:lang="en">birthPlace</rdfs:label>
    <skos:scopeNote xml:lang="en">Preferably, use a link to an existing thesaurus like geonames or wikidata.
                          If desired, both the literal place, as mentioned on the Source can be used together with
                          the reconciled version.
                       </skos:scopeNote>
    <sdo:domainIncludes rdf:resource="https://personsincontext.org/model/Person"/>
    <sdo:rangeIncludes rdf:resource="http://www.w3.org/2001/XMLSchema#string"/>
    <sdo:rangeIncludes rdf:resource="http://www.w3.org/2001/XMLSchema#anyURI"/>
  </rdf:Description>
  <rdf:Description rdf:about="https://personsincontext.org/model/hasStepsibling">
    <rdf:type rdf:resource="http://www.w3.org/2002/07/owl#ObjectProperty"/>
    <rdf:type rdf:resource="http://www.w3.org/2002/07/owl#SymmetricProperty"/>
    <rdfs:label xml:lang="en">hasStepsibling</rdfs:label>
    <rdfs:subPropertyOf rdf:resource="https://schema.org/relatedTo"/>
    <rdfs:domain rdf:resource="https://personsincontext.org/model/Person"/>
    <rdfs:range rdf:resource="https://personsincontext.org/model/Person"/>
  </rdf:Description>
  <rdf:Description rdf:about="https://personsincontext.org/model/hasParent-in-law">
    <rdf:type rdf:resource="http://www.w3.org/2002/07/owl#ObjectProperty"/>
    <rdfs:label xml:lang="en">hasParent-in-law</rdfs:label>
    <rdfs:subPropertyOf rdf:resource="https://schema.org/relatedTo"/>
    <rdfs:domain rdf:resource="https://personsincontext.org/model/Person"/>
    <rdfs:range rdf:resource="https://personsincontext.org/model/Person"/>
    <owl:inverseOf rdf:resource="https://personsincontext.org/model/hasChild-in-law"/>
  </rdf:Description>
  <rdf:Description rdf:about="https://schema.org/hasOccupation">
    <rdf:type rdf:resource="http://www.w3.org/2002/07/owl#DatatypeProperty"/>
    <rdfs:isDefinedBy rdf:resource="https://schema.org/hasOccupation"/>
    <skos:definition>The occupational title related to a person in an observation.</skos:definition>
    <rdfs:label xml:lang="en">hasOccupation</rdfs:label>
    <skos:scopeNote xml:lang="en">Todo</skos:scopeNote>
    <sdo:domainIncludes rdf:resource="https://personsincontext.org/model/PersonObservation"/>
    <sdo:rangeIncludes rdf:resource="http://www.w3.org/2001/XMLSchema#string"/>
    <sdo:rangeIncludes rdf:resource="http://www.w3.org/2001/XMLSchema#anyURI"/>
  </rdf:Description>
  <rdf:Description rdf:about="https://schema.org/familyName">
    <rdf:type rdf:resource="http://www.w3.org/2002/07/owl#DatatypeProperty"/>
    <rdfs:isDefinedBy rdf:resource="https://schema.org/familyName"/>
    <skos:definition>Family name. For Dutch names, this is the last name of a person.</skos:definition>
    <rdfs:label xml:lang="en">familyName</rdfs:label>
    <skos:scopeNote xml:lang="en">The use of sdo:givenName and sdo:familyName is the most straightforward method for
                          describing person names. Use pnv:Name for more extensive name annotations.
                       </skos:scopeNote>
    <sdo:domainIncludes rdf:resource="https://personsincontext.org/model/Person"/>
    <sdo:rangeIncludes rdf:resource="http://www.w3.org/2001/XMLSchema#string"/>
  </rdf:Description>
  <rdf:Description rdf:about="http://www.w3.org/ns/prov#wasRevisionOf">
    <rdf:type rdf:resource="http://www.w3.org/2002/07/owl#ObjectProperty"/>
    <rdfs:isDefinedBy rdf:resource="http://www.w3.org/ns/prov#wasRevisionOf"/>
    <skos:definition xml:lang="en">A revision is a derivation for which the resulting entity is a revised version of some
                          original.
                       </skos:definition>
    <rdfs:label xml:lang="en">wasRevisionOf</rdfs:label>
    <skos:scopeNote xml:lang="en">The wasRevisionOf property is used for modifications made on Person
                          reconstructions. It can be qualified with a prov:Revision.
                       </skos:scopeNote>
    <sdo:domainIncludes rdf:resource="https://personsincontext.org/model/PersonReconstruction"/>
    <sdo:rangeIncludes rdf:resource="https://personsincontext.org/model/PersonReconstruction"/>
  </rdf:Description>
  <rdf:Description rdf:about="https://w3id.org/pnv#literalName">
    <rdf:type rdf:resource="http://www.w3.org/2002/07/owl#DatatypeProperty"/>
    <rdfs:isDefinedBy rdf:resource="https://w3id.org/pnv#literalName"/>
    <skos:definition xml:lang="en">Literal name designates a full personal name. This property may only be left blank if a
                          person's name was unknown or if a person was unnamed (e.g. a child that died shortly after
                          being born), in which cases the property pnv:nameSpecification should state "unknown" or
                          "unnamed".
                       </skos:definition>
    <rdfs:label xml:lang="en">literalName</rdfs:label>
    <sdo:domainIncludes rdf:resource="https://w3id.org/pnv#Name"/>
    <sdo:rangeIncludes rdf:resource="http://www.w3.org/2001/XMLSchema#string"/>
  </rdf:Description>
  <rdf:Description rdf:about="https://w3id.org/pnv#givenName">
    <rdf:type rdf:resource="http://www.w3.org/2002/07/owl#DatatypeProperty"/>
    <rdfs:isDefinedBy rdf:resource="https://w3id.org/pnv#givenName"/>
    <skos:definition xml:lang="en">The given name of a pnv:Name. Designates the name(s) given to someone at birth or any other
                       name-giving event.
                       </skos:definition>
    <rdfs:label xml:lang="en">givenName (pnv)</rdfs:label>
    <sdo:domainIncludes rdf:resource="https://w3id.org/pnv#Name"/>
    <sdo:rangeIncludes rdf:resource="http://www.w3.org/2001/XMLSchema#string"/>
  </rdf:Description>
  <rdf:Description rdf:about="https://personsincontext.org/model/hasGrandparent">
    <rdf:type rdf:resource="http://www.w3.org/2002/07/owl#ObjectProperty"/>
    <rdfs:label xml:lang="en">hasGrandparent</rdfs:label>
    <rdfs:subPropertyOf rdf:resource="https://schema.org/relatedTo"/>
    <rdfs:domain rdf:resource="https://personsincontext.org/model/Person"/>
    <rdfs:range rdf:resource="https://personsincontext.org/model/Person"/>
    <owl:inverseOf rdf:resource="https://personsincontext.org/model/hasGrandchild"/>
  </rdf:Description>
  <rdf:Description rdf:about="https://personsincontext.org/model/hasStepparent-in-law">
    <rdf:type rdf:resource="http://www.w3.org/2002/07/owl#ObjectProperty"/>
    <rdfs:label xml:lang="en">hasStepparent-in-law</rdfs:label>
    <rdfs:subPropertyOf rdf:resource="https://schema.org/relatedTo"/>
    <rdfs:domain rdf:resource="https://personsincontext.org/model/Person"/>
    <rdfs:range rdf:resource="https://personsincontext.org/model/Person"/>
    <owl:inverseOf rdf:resource="https://personsincontext.org/model/hasStepchild-in-law"/>
  </rdf:Description>
  <rdf:Description rdf:about="https://w3id.org/pnv#Name">
    <rdf:type rdf:resource="http://www.w3.org/2002/07/owl#Class"/>
    <skos:definition xml:lang="en">Name of a person, expressed in Person Name Vocabulary (PNV)</skos:definition>
    <rdfs:label xml:lang="en">PersonName</rdfs:label>
    <skos:scopeNote xml:lang="en">In the Person Name Vocabulary, a name is considered to be a
                        a resource type in its own right.
                        A PersonName can consist of many different parts. The most common ones are mentioned here.
                        See the full specification of the Person Name Vocabulary for more details.
                        Additionally to a pnv:Name, the properties sdo:literalName or sdo:givenName and sdo:familyName should be used.
                      </skos:scopeNote>
  </rdf:Description>
  <rdf:Description rdf:about="https://schema.org/associatedMedia">
    <rdf:type rdf:resource="http://www.w3.org/2002/07/owl#ObjectProperty"/>
    <rdfs:isDefinedBy rdf:resource="https://schema.org/associatedMedia"/>
    <skos:definition xml:lang="en">A media object, usually a scan, that encodes the Source of a Person observation.</skos:definition>
    <rdfs:label xml:lang="en">associatedMedia</rdfs:label>
    <skos:scopeNote xml:lang="en">scopeNote
                             ...
                          </skos:scopeNote>
    <sdo:domainIncludes rdf:resource="https://schema.org/ArchiveComponent"/>
    <sdo:rangeIncludes rdf:resource="https://schema.org/ImageObject"/>
  </rdf:Description>
  <rdf:Description rdf:about="https://schema.org/children">
    <rdf:type rdf:resource="http://www.w3.org/2002/07/owl#ObjectProperty"/>
    <rdfs:isDefinedBy rdf:resource="https://schema.org/children"/>
    <skos:definition xml:lang="en">A child of a person.
                       </skos:definition>
    <rdfs:label xml:lang="en">children</rdfs:label>
    <skos:scopeNote xml:lang="en">For Person observations, the child should always refer to another Person observation
                             on the same Source.
                          </skos:scopeNote>
    <skos:scopeNote xml:lang="en">For Person reconstructions, the child should refer to another Person reconstruction.
                          </skos:scopeNote>
    <rdfs:subPropertyOf rdf:resource="https://schema.org/relatedTo"/>
    <rdfs:subPropertyOf rdf:resource="https://personsincontext.org/model/hasDescendant"/>
    <sdo:domainIncludes rdf:resource="https://personsincontext.org/model/Person"/>
    <sdo:rangeIncludes rdf:resource="https://personsincontext.org/model/Person"/>
    <owl:inverseOf rdf:resource="https://schema.org/parent"/>
  </rdf:Description>
  <rdf:Description rdf:about="https://personsincontext.org/model/hasGreat-grandchild">
    <rdf:type rdf:resource="http://www.w3.org/2002/07/owl#ObjectProperty"/>
    <rdfs:label xml:lang="en">hasGreat-grandchild</rdfs:label>
    <rdfs:subPropertyOf rdf:resource="https://schema.org/relatedTo"/>
    <rdfs:domain rdf:resource="https://personsincontext.org/model/Person"/>
    <rdfs:range rdf:resource="https://personsincontext.org/model/Person"/>
    <owl:inverseOf rdf:resource="https://personsincontext.org/model/hasGreat-grandparent"/>
  </rdf:Description>
  <rdf:Description rdf:nodeID="nf684994b51a046b584742dbc196ee550b1">
    <rdf:type rdf:resource="https://schema.org/ImageObject"/>
    <sh:order rdf:datatype="http://www.w3.org/2001/XMLSchema#integer">0</sh:order>
    <sdo:caption>Schematic overview</sdo:caption>
    <sdo:contentUrl rdf:datatype="http://www.w3.org/2001/XMLSchema#anyURI">../web_images/pico_overview.svg</sdo:contentUrl>
    <sdo:description>Schematic overview of the model.</sdo:description>
    <sdo:encodingFormat>image/svg+xml</sdo:encodingFormat>
    <sdo:name>Model overview</sdo:name>
  </rdf:Description>
  <rdf:Description rdf:about="https://schema.org/dateCreated">
    <rdf:type rdf:resource="http://www.w3.org/2002/07/owl#DatatypeProperty"/>
    <rdfs:isDefinedBy rdf:resource="https://schema.org/dateCreated"/>
    <skos:definition>The date on which the Source was created.</skos:definition>
    <rdfs:label xml:lang="en">dateCreated</rdfs:label>
    <sdo:domainIncludes rdf:resource="https://schema.org/ArchiveComponent"/>
    <sdo:rangeIncludes rdf:resource="http://www.w3.org/2001/XMLSchema#date"/>
  </rdf:Description>
  <rdf:Description rdf:about="https://personsincontext.org/model/hasAge">
    <rdf:type rdf:resource="http://www.w3.org/2002/07/owl#DatatypeProperty"/>
    <skos:definition xml:lang="en">The age of a person.</skos:definition>
    <rdfs:label xml:lang="en">hasAge</rdfs:label>
    <skos:scopeNote xml:lang="en">Only used for Person observations, in case the birth date is not known,
                                  but the age is. In combination with de date of the Source, a birth date range can
                                  be derived, which can be used in the process of creating a Person reconstruction.
                                  The age is considered to be in years, unless otherwise mentioned. So an age of
                                  "4" is considered to be 4 years, where "4 months" is interpreted as 4 months.
                                  Numerical ages ("4") are preferred above ages in text ("four").
                               </skos:scopeNote>
    <sdo:domainIncludes rdf:resource="https://personsincontext.org/model/PersonObservation"/>
    <sdo:rangeIncludes rdf:resource="http://www.w3.org/2001/XMLSchema#string"/>
  </rdf:Description>
  <rdf:Description rdf:about="https://personsincontext.org/model/hasNephew_Niece-in-law">
    <rdf:type rdf:resource="http://www.w3.org/2002/07/owl#ObjectProperty"/>
    <rdfs:label xml:lang="en">hasNephew-in-law/Niece-in-law</rdfs:label>
    <rdfs:subPropertyOf rdf:resource="https://schema.org/relatedTo"/>
    <rdfs:domain rdf:resource="https://personsincontext.org/model/Person"/>
    <rdfs:range rdf:resource="https://personsincontext.org/model/Person"/>
    <owl:inverseOf rdf:resource="https://personsincontext.org/model/hasUncle_Aunt-in-law"/>
  </rdf:Description>
  <rdf:Description rdf:about="https://schema.org/birthDate">
    <rdf:type rdf:resource="http://www.w3.org/2002/07/owl#DatatypeProperty"/>
    <rdfs:isDefinedBy rdf:resource="https://schema.org/birthDate"/>
    <skos:definition>The birth date of a persoon.</skos:definition>
    <rdfs:label xml:lang="en">birthDate</rdfs:label>
    <skos:scopeNote xml:lang="en">The birth date of a person. A date value in ISO 8601 format should be used.
                          Incomplete dates are allowed, but only when truncated from small to large. For example:
                          "1970-08-15", "1970-08" and "1970" are all allowed, but "1970-00-15" or "08-15" are not.
                          Sometimes, you may want use a string as birthDate. For example if you want to or have to
                          record the date exactly as it was written on the Source. If possible use both the string
                          format and the xsd:date format in this case.
                       </skos:scopeNote>
    <sdo:domainIncludes rdf:resource="https://personsincontext.org/model/Person"/>
    <sdo:rangeIncludes rdf:resource="http://www.w3.org/2001/XMLSchema#date"/>
    <sdo:rangeIncludes rdf:resource="http://www.w3.org/2001/XMLSchema#string"/>
  </rdf:Description>
  <rdf:Description rdf:about="https://schema.org/parent">
    <rdf:type rdf:resource="http://www.w3.org/2002/07/owl#ObjectProperty"/>
    <rdfs:isDefinedBy rdf:resource="https://schema.org/parent"/>
    <skos:definition>A parent of a person.</skos:definition>
    <rdfs:label xml:lang="en">parent</rdfs:label>
    <skos:scopeNote xml:lang="en">For Person observations, the parent should always refer to another Person observation
                          on the same Source. For Person reconstructions, the parent should refer to another Person
                          reconstruction.
                       </skos:scopeNote>
    <rdfs:subPropertyOf rdf:resource="https://schema.org/relatedTo"/>
    <rdfs:subPropertyOf rdf:resource="https://personsincontext.org/model/hasAncestor"/>
    <sdo:domainIncludes rdf:resource="https://personsincontext.org/model/Person"/>
    <sdo:rangeIncludes rdf:resource="https://personsincontext.org/model/Person"/>
    <owl:inverseOf rdf:resource="https://schema.org/children"/>
  </rdf:Description>
  <rdf:Description rdf:nodeID="nf684994b51a046b584742dbc196ee550b6">
    <rdf:type rdf:resource="https://schema.org/TextObject"/>
    <sdo:description>Example of a Person Reconstruction</sdo:description>
    <sdo:encodingFormat>text/turtle</sdo:encodingFormat>
    <sdo:name>Person Reconstruction example</sdo:name>
    <sdo:text>
                                                cbg:person_reconstruction_2
                                                    a                   pico:PersonReconstruction ;
                                                    sdo:name            "Anna Maria Koppen" ;
                                                    sdo:familyName      "Koppen" ;
                                                    sdo:givenName       "Anna" ;
                                                    sdo:gender          sdo:Female ;
                                                    sdo:birthPlace      "Haarlem" ;
                                                    sdo:birthDate       "1860-03-31"^^xsd:date ;
                                                    sdo:deathPlace      "Detroit, VSA" ;
                                                    sdo:deathDate       "1926"^^xsd:gYear ;
                                                    prov:wasDerivedFrom nha:huwelijksakte_1885_321_po_1, cbg:NL-HaCBG_1755_0341_142_po_1 ;
                                                    prov:wasGeneratedBy cbg:reconstruction_activity_01 .

                                                cbg:reconstruction_activity_01
                                                    a                      prov:Activity ;
                                                    prov:wasAssociatedWith cbg:reconstruction_agent_01 ;
                                                    prov:startedAtTime     "2015-08-07T00:00:00"^^xsd:dateTime ;
                                                    prov:endedAtTime       "2020-01-08T00:00:00"^^xsd:dateTime .
                                                </sdo:text>
  </rdf:Description>
  <rdf:Description rdf:about="https://w3id.org/pnv#surnamePrefix">
    <rdf:type rdf:resource="http://www.w3.org/2002/07/owl#DatatypeProperty"/>
    <rdfs:isDefinedBy rdf:resource="https://w3id.org/pnv#surnamePrefix"/>
    <skos:definition xml:lang="en">A Surname prefix is a name part prefixing the surname (e.g. 'van' or 'van den').
                       </skos:definition>
    <rdfs:label xml:lang="en">surnamePrefix</rdfs:label>
    <skos:scopeNote xml:lang="en">A2A:PersonNamePrefixLastName</skos:scopeNote>
    <sdo:domainIncludes rdf:resource="https://w3id.org/pnv#Name"/>
    <sdo:rangeIncludes rdf:resource="http://www.w3.org/2001/XMLSchema#string"/>
  </rdf:Description>
  <rdf:Description rdf:about="https://personsincontext.org/model/hasChild-in-law">
    <rdf:type rdf:resource="http://www.w3.org/2002/07/owl#ObjectProperty"/>
    <rdfs:label xml:lang="en">hasChild-in-law</rdfs:label>
    <rdfs:subPropertyOf rdf:resource="https://schema.org/relatedTo"/>
    <rdfs:domain rdf:resource="https://personsincontext.org/model/Person"/>
    <rdfs:range rdf:resource="https://personsincontext.org/model/Person"/>
    <owl:inverseOf rdf:resource="https://personsincontext.org/model/hasParent-in-law"/>
  </rdf:Description>
  <rdf:Description rdf:about="https://personsincontext.org/model/hasGrandchild-in-law">
    <rdf:type rdf:resource="http://www.w3.org/2002/07/owl#ObjectProperty"/>
    <rdfs:label xml:lang="en">hasGrandchild-in-law</rdfs:label>
    <rdfs:subPropertyOf rdf:resource="https://schema.org/relatedTo"/>
    <rdfs:domain rdf:resource="https://personsincontext.org/model/Person"/>
    <rdfs:range rdf:resource="https://personsincontext.org/model/Person"/>
    <owl:inverseOf rdf:resource="https://personsincontext.org/model/hasGrandparent-in-law"/>
  </rdf:Description>
  <rdf:Description rdf:about="https://personsincontext.org/model/hasStepparent">
    <rdf:type rdf:resource="http://www.w3.org/2002/07/owl#ObjectProperty"/>
    <rdfs:label xml:lang="en">hasStepparent</rdfs:label>
    <rdfs:subPropertyOf rdf:resource="https://schema.org/relatedTo"/>
    <rdfs:domain rdf:resource="https://personsincontext.org/model/Person"/>
    <rdfs:range rdf:resource="https://personsincontext.org/model/Person"/>
    <owl:inverseOf rdf:resource="https://personsincontext.org/model/hasStepchild"/>
  </rdf:Description>
  <rdf:Description rdf:about="https://personsincontext.org/model/deceased">
    <rdf:type rdf:resource="http://www.w3.org/2002/07/owl#DatatypeProperty"/>
    <skos:definition>Indication if a person is deceased.</skos:definition>
    <rdfs:label xml:lang="en">deceased</rdfs:label>
    <skos:scopeNote xml:lang="en">Indication if a person is still alive or not at time of the source of the observation.
                             Only used when deathDate is unknown.
                             A person without a deathDate and without the property deceased set to true,
                             will be considered alive. This will have consequences for the publication
                             of the person record and of any linked media items.
                          </skos:scopeNote>
    <sdo:domainIncludes rdf:resource="https://personsincontext.org/model/PersonObservation"/>
    <sdo:rangeIncludes rdf:resource="http://www.w3.org/2001/XMLSchema#boolean"/>
  </rdf:Description>
  <rdf:Description rdf:about="https://personsincontext.org/model/hasStepchild">
    <rdf:type rdf:resource="http://www.w3.org/2002/07/owl#ObjectProperty"/>
    <rdfs:label xml:lang="en">hasStepchild</rdfs:label>
    <rdfs:subPropertyOf rdf:resource="https://schema.org/relatedTo"/>
    <rdfs:domain rdf:resource="https://personsincontext.org/model/Person"/>
    <rdfs:range rdf:resource="https://personsincontext.org/model/Person"/>
    <owl:inverseOf rdf:resource="https://personsincontext.org/model/hasStepparent"/>
  </rdf:Description>
  <rdf:Description rdf:about="https://terms.personsincontext.org/sourectypes">
    <rdf:type rdf:resource="http://www.w3.org/2004/02/skos/core#ConceptScheme"/>
    <rdfs:label>Persons in Context sourceType thesaurus</rdfs:label>
  </rdf:Description>
  <rdf:Description rdf:about="https://schema.org/givenName">
    <rdf:type rdf:resource="http://www.w3.org/2002/07/owl#DatatypeProperty"/>
    <rdfs:isDefinedBy rdf:resource="https://schema.org/givenName"/>
    <skos:definition>Given name. For Dutch names, this could be multiple given names of a person.</skos:definition>
    <rdfs:label>givenName (schema)</rdfs:label>
    <skos:scopeNote xml:lang="en">The use of sdo:givenName and sdo:familyName is the preferred method for
                             describing person names. Use pnv:Name for more extensive name annotations.
                          </skos:scopeNote>
    <sdo:domainIncludes rdf:resource="https://personsincontext.org/model/Person"/>
    <sdo:rangeIncludes rdf:resource="http://www.w3.org/2001/XMLSchema#string"/>
  </rdf:Description>
</rdf:RDF>
